\documentclass[12pt]{article}
\usepackage{pmmeta}
\pmcanonicalname{ProofOfSilvermanToeplitzTheorem}
\pmcreated{2013-03-22 14:51:35}
\pmmodified{2013-03-22 14:51:35}
\pmowner{rspuzio}{6075}
\pmmodifier{rspuzio}{6075}
\pmtitle{proof of Silverman-Toeplitz theorem}
\pmrecord{27}{36533}
\pmprivacy{1}
\pmauthor{rspuzio}{6075}
\pmtype{Proof}
\pmcomment{trigger rebuild}
\pmclassification{msc}{40B05}

\endmetadata

% this is the default PlanetMath preamble.  as your knowledge
% of TeX increases, you will probably want to edit this, but
% it should be fine as is for beginners.

% almost certainly you want these
\usepackage{amssymb}
\usepackage{amsmath}
\usepackage{amsfonts}

% used for TeXing text within eps files
%\usepackage{psfrag}
% need this for including graphics (\includegraphics)
%\usepackage{graphicx}
% for neatly defining theorems and propositions
%\usepackage{amsthm}
% making logically defined graphics
%%%\usepackage{xypic}

% there are many more packages, add them here as you need them

% define commands here
\begin{document}
First, we shall show that the series $\sum_{n=0}^\infty a_{mn} z_n$ converges.  Since the sequence $\{z_n\}$ converges, it must be bounded in absolute value --- there must exist a constant $K > 0$ 
such that $|z_n| \le K$ for all $n$.  Hence,  $|a_{mn} z_n| \le K |a_{mn}|.$  Summing this gives
 $$\sum_{n=0}^\infty |a_{mn} z_n| \le K \sum_{n=0}^\infty |a_{mn}| \le KB.$$
Hence, the series $\sum_{n=0}^\infty a_{mn} z_n$ is absolutely convergent which, in turn, implies that it converges.

 Let $z$ denote the limit of the sequence $\{z_n\}$ as $n \to \infty$. Then $\vert z \vert \le K$.
 We need to show that, for every $\epsilon > 0$, there exists an integer $M$ such that
 $$\left| \sum_{n=0}^\infty a_{mn} z_n - z \right| < \epsilon$$
whenever $m > M$.

Since the sequence $\{z_n\}$ converges, there must exist an integer $n_1$ such that
 $|z_n - z| < \frac{\epsilon}{4B}$ whenever $n > n_1$.  

By condition 3, there must exist constants $m_o,m_1,  \ldots , m_{n_1}$ such that 
\begin{equation}
|a_{mn}| < {\epsilon \over 4 (n_1 +1)(K+1)} \quad \textrm{for} \quad  0 \le n \le n_1 \quad \textrm{and} \quad  m > m_n.
\end{equation}
  
Choose $m'= \max\{ m_0,m_1,  \ldots, m_{n_1} \}.$  Then 
\begin{equation}
\left| \sum_{n=0}^{n_1} a_{mn} z_n \right| \le \sum_{n=0}^{n_1} |a_{mn} z_n| < \sum_{n=0}^{n_1} {|z_n| \epsilon \over 4 (n_1+1) (K+1)} < {\epsilon \over 4}
\end{equation}
when $m > m'.$

By condition 2, there  exists a constant $m''$ such that
 $$\left| \sum_{n=0}^\infty a_{mn} - 1 \right| < {\epsilon \over 6 (|z|+1)}$$
whenever $m > m''$.  By (1),
 $$\left| \sum_{n=0}^{n_1} a_{mn} \right| < {\epsilon \over 4(K+1)} \le {\epsilon \over 4(|z|+1)}$$
when $m > m'$.  Hence, if $m > m'$ and $m > m''$, we have
\begin{equation}
\left| \sum_{n=n_1 + 1}^\infty a_{mn} - 1 \right| < {\epsilon \over 2(|z|+1)}.
\end{equation}

and
\begin{equation}
 \left| \sum_{n=n_1 + 1}^\infty a_{mn} (z_n - z) \right| \le \sum_{n=n_1 + 1}^\infty |a_{mn}| ~ |z_n - z| < {\epsilon \over 4B} \sum_{n=0}^\infty |a_{mn}| \le {\epsilon \over 4}.
\end{equation}
By the triangle inequality and (2), (3), (4) it follows that
 $$\left| \sum_{n=0}^\infty a_{mn} z_n - z \right| \le \left| \sum_{n=0}^{n_1} a_{mn} z_n \right| + \left| \sum_{n=n_1 + 1}^\infty a_{mn} (z_n - z) \right| + |z| \left| \sum_{n=n_1 + 1}^\infty a_{mn} - 1 \right|$$
$$ 
< \frac{\epsilon}{4} + \frac{\epsilon}{4} + \frac{\epsilon}{2} = \epsilon.
$$


%%%%%
%%%%%
\end{document}
